src/ReactorModel/Objects/Reactor/Finite.lean
@@ -1,0 +1,18 @@
+import ReactorModel.Objects.Reactor.Indexable
+
+noncomputable section
+
+namespace ReactorType
+
+class Finite (α) extends Indexable α where
+  fin : ∀ (rtr : α) (cpt : Component), rtr[cpt].Finite
+
+namespace Finite
+
+variable [Finite α]
+
+def ids (rtr : α) (cpt : Component) : List cpt.idType :=
+  (fin rtr cpt).toFinset.toList 
+
+end Finite
+namespace ReactorType
