src/ReactorModel/Objects/Reactor/Practical.lean
@@ -1,0 +1,8 @@
+import ReactorModel.Objects.Reactor.Finite
+import ReactorModel.Objects.Reactor.Proper
+
+namespace ReactorType
+
+class Practical (α) extends Finite α, Proper α  
+
+end ReactorType
