src/ReactorModel/Objects/Reactor/Theorems/FiniteUpdatable.lean
@@ -1,0 +1,38 @@
+import ReactorModel.Objects.Reactor.Practical
+import ReactorModel.Objects.Reactor.Theorems.Indexable
+
+noncomputable section
+
+namespace ReactorType
+
+class FiniteUpdatable (α) extends Finite α, LawfulUpdatable α
+
+instance [Practical α] : FiniteUpdatable α where
+  update := Practical.update
+  lawful := Practical.lawful
+
+namespace FiniteUpdatable
+
+variable [FiniteUpdatable α]
+
+def update' (rtr : α) (cpt : Component.Valued) (v : cpt.type) : α :=
+  go rtr cpt v $ Finite.ids rtr cpt
+where 
+  go (rtr : α) (cpt : Component.Valued) (v : cpt.type) : List ID → α
+  | [] => rtr
+  | hd :: tl => go (update rtr cpt hd fun _ => v) cpt v tl
+
+variable {rtr : α} 
+
+theorem update'.go_equiv (ids : List ID) : rtr ≈ update'.go rtr cpt v ids := by
+  induction ids generalizing rtr <;> simp [go]
+  case nil => sorry -- exact .refl _ TODO: Update ReactorType.Equivalent with refl as constructor.
+  case cons hd _ hi => 
+    have : rtr ≈ update rtr cpt hd fun _ => v := sorry -- exact LawfulUpdatable.equiv TODO: Update ReactorType.Equivalent with refl as constructor.
+    exact Equivalent.trans this hi
+
+theorem update'_equiv : rtr ≈ update' rtr cpt v :=
+  update'.go_equiv _
+
+end FiniteUpdatable
+end ReactorType
