src/ReactorModel/Objects/Reactor/Theorems/WellUpdatable.lean
@@ -6,7 +6,7 @@ class WellUpdatable (α) extends LawfulUpdatable α, WellFounded α
 
 variable [WellUpdatable α] {rtr : α}
 
-theorem LawfulUpdatable.equiv : (Updatable.update rtr cpt i f) ≈ rtr := 
-  Equivalent.symm (lawful rtr cpt i f).equiv
+theorem LawfulUpdatable.equiv : rtr ≈ (Updatable.update rtr cpt i f) := 
+  (lawful rtr cpt i f).equiv
 
 end ReactorType
